some of sub-lemma proof...hard parts to do...

Ref-STLC.v
@@ -12,6 +12,8 @@ Require Coq.Structures.Equalities.
 Module SE := Coq.Structures.Equalities.
 Require Coq.FSets.FMapWeakList.
 Module FM := Coq.FSets.FMapWeakList.
+Require Coq.FSets.FMapFacts.
+Module FF := Coq.FSets.FMapFacts.
 Require Import Coq.Arith.PeanoNat.
 Require Coq.MSets.MSetWeakList.
 Module WS := Coq.MSets.MSetWeakList.
@@ -22,6 +24,14 @@ Inductive type : Type :=
     | TUnit
     | TFun : type -> type -> type
     | TRef : type -> type.
+
+Fixpoint type_eqb (a b : type) : bool :=
+    match a, b with
+    | TUnit, TUnit => true 
+    | TFun a1 a2, TFun b1 b2 => type_eqb a1 b1 && type_eqb a2 b2
+    | TRef a, TRef b => type_eqb a b
+    | _, _ => false
+    end.
 
 Definition id := string.
 
@@ -63,6 +73,8 @@ End IdDec.
 
 Module IM := FM.Make(IdDec).
 
+Module IFF := FF.WFacts_fun(IdDec)(IM).
+
 (* typing context *)
 Definition gamma := IM.t type.
 
@@ -85,6 +97,8 @@ End LocDec.
 
 Module LM := FM.Make(LocDec).
 
+Module LF := FF.WFacts_fun(LocDec)(LM).
+
 (* evaluation stores *)
 Definition mu : Type := LM.t expr.
 
@@ -94,7 +108,7 @@ Definition sigma : Type := LM.t type.
 (* Static Semantics *)
 Inductive check (g : gamma) (s : sigma) : expr -> type -> Prop :=
     | check_var : forall (x : id) (t : type), 
-        IM.find x g = Some t ->
+        IM.MapsTo x t g ->
         check g s (EVar x) t
     | check_fun : forall (x : id) (t t' : type) (e : expr),
         check (IM.add x t g) s e t' ->
@@ -135,47 +149,47 @@ Fixpoint fv (e : expr) : IS.t :=
     end.
 
 (* Capture-avoiding Substitution *)
-Inductive sub (x : id) (s : expr) : expr -> expr -> Prop :=
-    | sub_hit : sub x s (EVar x) s
+Inductive sub (x : id) (es : expr) : expr -> expr -> Prop :=
+    | sub_hit : sub x es (EVar x) es
     | misssub : forall (y : id), 
-        y <> x -> 
-        sub x s (EVar y) (EVar y)
+        x <> y -> 
+        sub x es (EVar y) (EVar y)
     | sub_fun_bound : forall (t : type) (e : expr),
-        sub x s (EFun x t e) (EFun x t e)
+        sub x es (EFun x t e) (EFun x t e)
     | sub_lam_notfree : forall (y : string) (t : type) (e e' : expr),
         x <> y ->
-         ~ IS.In y (fv s) -> 
-        sub x s e e' -> 
-        sub x s (EFun y t e) (EFun y t e')
+         ~ IS.In y (fv es) -> 
+        sub x es e e' -> 
+        sub x es (EFun y t e) (EFun y t e')
     | sub_lam_free : forall (y z : id) (t : type) (e e' e'' : expr),
         x <> y -> 
         x <> z -> 
         y <> z ->
-        IS.In y (fv s) -> 
-        ~ IS.In z (fv s) ->
+        IS.In y (fv es) -> 
+        ~ IS.In z (fv es) ->
         ~ IS.In z (fv e) ->
         sub y (EVar z) e e' -> 
-        sub x s e' e'' -> 
-        sub x s (EFun y t e) (EFun z t e'')
+        sub x es e' e'' -> 
+        sub x es (EFun y t e) (EFun z t e'')
     | sub_app : forall (e1 e1' e2 e2' : expr),
-        sub x s e1 e1' -> 
-        sub x s e2 e2' -> 
-        sub x s (EApp e1 e2) (EApp e1' e2')
-    | sub_unit : sub x s EUnit EUnit
+        sub x es e1 e1' -> 
+        sub x es e2 e2' -> 
+        sub x es (EApp e1 e2) (EApp e1' e2')
+    | sub_unit : sub x es EUnit EUnit
     | sub_ref : forall (e e' : expr),
-        sub x s e e' ->
-        sub x s (ERef e) (ERef e')
+        sub x es e e' ->
+        sub x es (ERef e) (ERef e')
     | sub_bang : forall (e e' : expr),
-        sub x s e e' ->
-        sub x s (EBang e) (EBang e')
+        sub x es e e' ->
+        sub x es (EBang e) (EBang e')
     | sub_ass : forall (e1 e1' e2 e2' : expr),
-        sub x s e1 e1' ->
-        sub x s e2 e2' ->
-        sub x s (EAss e1 e2) (EAss e1' e2')
+        sub x es e1 e1' ->
+        sub x es e2 e2' ->
+        sub x es (EAss e1 e2) (EAss e1' e2')
     | sub_loc : forall (l : loc),
-        sub x s (ELoc l) (ELoc l).
+        sub x es (ELoc l) (ELoc l).
 
-Axiom sub_exists : forall (x : string) (s e : expr), exists e', sub x s e e'.
+Axiom sub_exists : forall (x : string) (es e : expr), exists e', sub x es e e'.
 
 (* Dynamic Semantics *)
 Inductive step (m : mu) : expr -> expr -> mu -> Prop :=
@@ -189,7 +203,7 @@ Inductive step (m : mu) : expr -> expr -> mu -> Prop :=
         ~ LM.In l m ->
         step m (ERef e) (ELoc l) (LM.add l e m)
     | step_loc : forall (l : loc) (e : expr),
-        LM.find l m = Some e ->
+        LM.MapsTo l e m ->
         step m (EBang (ELoc l)) e m
     | step_bang : forall (e e' : expr) (m' : mu),
         step m e e' m' ->
@@ -199,3 +213,100 @@ Inductive step (m : mu) : expr -> expr -> mu -> Prop :=
     | step_ass2 : forall (e1 e1' e2 : expr) (m' : mu),
         step m e1 e1' m' ->
         step m (EAss e1 e2) (EAss e1' e2) m'.
+
+Definition subset (s s' : sigma) :=
+    forall (l : loc) (t : type), LM.MapsTo l t s -> LM.MapsTo l t s'.
+
+Lemma mu_monotonic :
+    forall (g : gamma) (s s' : sigma) (e : expr) (t : type),
+    check g s e t -> subset s s' -> check g s' e t.
+Proof.
+    intros. dependent induction H;
+    try constructor; try assumption; auto.
+    - eapply check_app; auto.
+    - eapply check_ass; auto.
+    - eapply LF.find_mapsto_iff. apply H0. 
+        eapply LF.find_mapsto_iff. assumption.
+Qed.
+
+Definition dom_eq {A B : Type} (fa : LM.t A) (fb : LM.t B) : Prop :=
+    forall (l : loc), LM.In l fa <-> LM.In l fb.
+
+Definition well_typed_ctxts (m : mu) (s : sigma) (g : gamma) : Prop :=
+    dom_eq m s /\ forall (l : loc) (e : expr) (t : type), 
+        LM.MapsTo l e m ->
+        LM.MapsTo l t s ->
+        check g s e t.
+
+Definition preservation 
+    (g : gamma) (s : sigma) (e e' : expr) (m m' : mu) (t : type) : Prop := 
+    step m e e' m' ->
+    well_typed_ctxts m s g ->
+    check g s e t ->
+    forall (s' : sigma), subset s s' ->
+    well_typed_ctxts m' s' g /\ check g s' e' t.
+
+Definition substitution_lemma 
+    (x : id) (e1 e1' e2 : expr) : Prop := 
+    sub x e2 e1 e1' ->
+    forall (g : gamma) (s : sigma) (a b : type),
+    check (IM.add x a g) s e1 b -> 
+    check g s e2 a ->
+    check g s e1' b.
+
+Axiom add_twice : 
+    forall {T : Type} (x : id) (a b : T) (map : IM.t T),
+    IM.add x a (IM.add x b map) = IM.add x a map.
+
+Theorem substitution_lemma_holds : 
+    forall (x : id) (e1 e1' e2 : expr),
+    substitution_lemma x e1 e1' e2.
+Proof.
+    unfold substitution_lemma.
+    intros x e1 e1' e2 HS.
+    induction HS; intros.
+    - inversion H; subst.
+        apply IFF.add_mapsto_iff in H2 as [[_ AB] | [HMT _]]; 
+        subst; auto. contradiction.
+    - inversion H0; subst. constructor. eapply IM.add_3 in H.
+        + apply H.
+        + apply H3.
+    - inversion H; subst. constructor. 
+        rewrite add_twice in H5. assumption.
+    - inversion H1; subst. constructor.
+        specialize IHHS with 
+            (g := g) (s := s) (a := a) (b := t').
+            admit.
+    - inversion H5; subst. admit.
+    - inversion H; subst. eapply check_app.
+        + eapply IHHS1.
+            * apply H3.
+            * assumption.
+        + eapply IHHS2.
+            * apply H5.
+            * assumption.
+    - inversion H; subst. constructor.
+    - inversion H; subst. 
+        constructor. eapply IHHS.
+        + apply H2.
+        + assumption.
+    - inversion H; subst.
+        constructor. eapply IHHS.
+        + apply H2.
+        + assumption.
+    - inversion H; subst.
+        eapply check_ass.
+        + eapply IHHS1.
+            * apply H3.
+            * assumption.
+        + eapply IHHS2.
+            * apply H5.
+            * assumption.
+    - inversion H; subst.
+        constructor. assumption.
+Admitted.
+
+
+
+
+
